\documentclass[a4paper,11pt]{article}
\usepackage{braket}
\usepackage{physics}
\usepackage{parskip}
\usepackage{bm}
\usepackage{float}
\usepackage[utf8]{inputenc}
\usepackage{amsmath}
\usepackage{pgfplots}
\usepackage{mathrsfs}
\usepackage{simpler-wick}
\usepackage{enumerate}
\usepackage{csquotes}
\usepackage{subcaption}
\usepackage{fancyhdr}
\usepackage{tablefootnote}
\usepackage{microtype}
\usepackage{cleveref}
\usepackage{titling}
\usepackage{erewhon}
\usepackage[a4paper,width=150mm,top=25mm,bottom=25mm]{geometry}
\usepackage[Sonny]{fncychap}
\usepackage[calcwidth]{titlesec}
\usepackage[makeroom]{cancel}

\usetikzlibrary{shapes.geometric, arrows}

\allowdisplaybreaks

\pgfplotsset{compat=1.7}

%fncychap layout (for chapter page)
%\renewcommand{\thechapter}{\Roman{chapter}}
\ChNameVar{\bfseries\LARGE\fontfamily{phv}}
\ChNumVar{\fontsize{50}{52}\usefont{OT1}{ptm}{m}{n}\selectfont}
\ChTitleVar{\LARGE\rm\bfseries}
\ChRuleWidth{0.8pt}

%fancyhdr layout (for header and footer)
\pagestyle{fancy}
\fancyhead{}
\fancyhead[C]{\fontsize{9}{9}\itshape{\rightmark}}
\setlength{\headheight}{15pt}

\begin{document}
\section{Direct Differentiation}
MP2 energy in spin-orbital formalism:
\begin{align}
    E ^{(2)} =& \frac{1}{4}\sum_{ijab}\frac{\langle ab||ij\rangle \langle ij||ab\rangle}{f _{ii}+f _{jj}-f _{aa}-f _{bb}} \nonumber \\
    =& \frac{1}{4}\sum_{ijab}T _{ij}^{ab}\langle ij||ab\rangle
\end{align}
in which we denote the MP2 amplitude:
\begin{equation}
    T _{ij}^{ab} = \frac{\langle ab||ij\rangle}{\Delta _{ab}^{ij}} = \frac{\langle ab||ij\rangle}{f _{ii}+f _{jj}-f _{aa}-f _{bb}}
\end{equation} 
Directly differentiate the second-order energy w.r.t. perturbation parameter $\lambda$:
\begin{align}
    \pdv{E ^{(2)}}{\lambda} =& \frac{1}{4}\sum_{ijab}\pdv{\lambda}(T _{ij}^{ab}\langle ij||ab\rangle) \nonumber \\
    =&\frac{1}{4}\sum_{ijab}\Big(\pdv{T _{ij}^{ab}}{\lambda}\Big)\langle ij||ab\rangle + \frac{1}{4}\sum_{ijab}T _{ij}^{ab} \Big(\pdv{\langle ij||ab\rangle}{\lambda}\Big)
\end{align}
in which:
\begin{align}
    \pdv{\langle ij||ab\rangle}{\lambda} = \langle i ^{\lambda}j||ab\rangle + \langle ij ^{\lambda}||ab\rangle + \langle ij||a ^{\lambda}b\rangle + \langle ij||ab ^{\lambda}\rangle
\end{align} 
exploiting the permutational symmetry and equivalence of the dummy indices:
\begin{align}
    \sum_{ijab}\langle ij ^{\lambda}||ab\rangle = \sum_{ijab}\langle j ^{\lambda}i||ba\rangle = \sum_{jiba}\langle i ^{\lambda}j||ab\rangle
\end{align}
Therefore:
\begin{equation}
    \sum_{ijab}\langle ij||ab\rangle ^{\lambda} = 2 \sum_{ijab}(\langle i ^{\lambda}j||ab\rangle + \langle ij||a ^{\lambda}b\rangle)
\end{equation}
Then:
\begin{align}
    \pdv{T _{ij}^{ab}}{\lambda} =& \pdv{\lambda}(\frac{\langle ab||ij\rangle}{\Delta _{ab}^{ij}}) \nonumber \\
    =& \frac{\langle ab||ij\rangle ^{\lambda}}{\Delta _{ab}^{ij}} - \frac{\langle ab||ij\rangle}{(\Delta _{ab}^{ij})^{2}}\Big(\pdv{\Delta _{ab}^{ij}}{\lambda}\Big) \nonumber \\
    =&  \frac{\langle ab||ij\rangle ^{\lambda}}{\Delta _{ab}^{ij}} - \frac{\langle ab||ij\rangle}{(\Delta _{ab}^{ij})^{2}}(\varepsilon _{i} ^{\lambda} + \varepsilon _{j}^{\lambda} - \varepsilon _{a}^{\lambda}-\varepsilon _{b}^{\lambda})
\end{align}
Putting eqns (6) and (7) together:
\begin{align}
    \pdv{E ^{(2)}}{\lambda} =& \frac{1}{4}\sum_{ijab}\langle ij||ab\rangle (T _{ij}^{ab})^{\lambda} + \frac{1}{4}\sum_{ijab}T _{ij}^{ab}\langle ij||ab\rangle ^{\lambda} \nonumber \\
    =& \frac{1}{4}\sum_{ijab}\langle ij||ab\rangle\Big(\frac{\langle ab||ij\rangle ^{\lambda}}{\Delta _{ab}^{ij}}-\frac{\langle ab||ij\rangle}{(\Delta _{ab}^{ij})^{2}}(\varepsilon _{i} ^{\lambda} + \varepsilon _{j}^{\lambda} - \varepsilon _{a}^{\lambda}-\varepsilon _{b}^{\lambda})\Big) + \frac{1}{4}\sum_{ijab}\langle ij||ab\rangle ^{\lambda}T _{ij} ^{ab} \nonumber \\
    =& \frac{1}{4}\sum_{ijab}\frac{\langle ij||ab\rangle\langle ab||ij\rangle ^{\lambda}}{\Delta _{ab}^{ij}} + \frac{1}{4}\sum_{ijab}\frac{\langle ij||ab\rangle ^{\lambda}\langle ab||ij\rangle}{\Delta _{ab}^{ij}}- \frac{1}{4}\sum_{ijab}\frac{\langle ij||ab\rangle\langle ab||ij\rangle}{(\Delta _{ab}^{ij})^{2}}(2 \varepsilon _{i}^{\lambda} -2 \varepsilon _{a}^{\lambda})  \nonumber \\
    =& \frac{1}{2}\sum_{ijab}(T _{ij}^{ab})^{*}\langle a ^{\lambda}b||ij\rangle + \frac{1}{2}\sum_{ijab}(T _{ij}^{ab})^{*}\langle ab||i ^{\lambda}j\rangle + \frac{1}{2}\sum_{ijab}T ^{ab}_{ij}\langle i ^{\lambda}j||ab\rangle + \frac{1}{2}\sum_{ijab} T _{ij}^{ab}\langle ij||a ^{\lambda}b\rangle \nonumber \\
    &- \frac{1}{2}\sum_{ijab}T _{ij}^{ab}(T _{ij}^{ab})^{*}(\varepsilon _{i}^{\lambda}-\varepsilon _{a}^{\lambda})
\end{align}
Using the expression for $|i ^{\lambda}\rangle$ and $|a ^{\lambda}\rangle$:
\begin{align}
    \pdv{E ^{(2)}}{\lambda}=& \frac{1}{2}\sum_{ijab}(T _{ij}^{ab})^{*}\Big(\sum_{k}(U _{ka}^{\lambda})^{*}\langle kb||ij\rangle + \sum_{f\neq a}(U _{fa}^{\lambda})^{*}\langle fb||ij\rangle + \sum_{\mu}C _{\mu a}^{*}\langle \mu ^{\lambda} b||ij\rangle\Big) \nonumber \\
    &+ \frac{1}{2}\sum_{ijab}(T _{ij}^{ab})^{*}\Big(\sum_{k\neq i}U _{ki}^{\lambda}\langle ab||kj\rangle + \sum_{f}U _{fi}^{\lambda}\langle ab||fj\rangle + \sum_{\mu}C _{\mu i}\langle ab||\mu ^{\lambda} j\rangle\Big) \nonumber \\
    &+ \frac{1}{2}\sum_{ijab}T _{ij}^{ab}\Big(\sum_{k\neq i}(U _{ki}^{\lambda})^{*}\langle kj||ab\rangle + \sum_{f}(U _{fi}^{\lambda})^{*}\langle fj||ab\rangle + \sum_{\mu}C _{\mu i}^{*}\langle \mu ^{\lambda} j||ab\rangle\Big) \nonumber \\
    &+ \frac{1}{2}\sum_{ijab}T _{ij}^{ab}\Big(\sum_{k}U _{ka}^{\lambda}\langle ij||kb\rangle + \sum_{f\neq a}U _{fa}^{\lambda}\langle ij||fb\rangle + \sum_{\mu}C _{\mu a}\langle ij||\mu ^{\lambda}b\rangle\Big) \nonumber \\
    &-\frac{1}{2}\sum_{ijab}T _{ij}^{ab}(T _{ij}^{ab})^{*}(\varepsilon _{i}^{\lambda}-\varepsilon _{a}^{\lambda})
\end{align}
Using the orthonormality condition on $(U _{ka}^{\lambda})^{*}$, $(U _{fa}^{\lambda})^{*}$, $(U _{ki}^{\lambda})^{*}$ and $U _{ka}^{\lambda}$, and omitting the AO terms (terms involving $|\phi _{\mu}\rangle$) for now:
\begin{align}
    \pdv{E ^{(2)}}{\lambda} =& \frac{1}{2}\sum_{ijab}\sum_{k}(T ^{ab}_{ij})^{*}\langle kb||ij\rangle(-S _{ak}^{\lambda} - U _{ak}^{\lambda}) + \frac{1}{2}\sum_{ijab}\sum_{f\neq a}(T _{ij}^{ab})^{*}\langle fb||ij\rangle(-S _{af}^{\lambda}-U _{af}^{\lambda}) \nonumber \\
    &+ \frac{1}{2}\sum_{ijab}\sum_{k\neq i}(T _{ij}^{ab})^{*}\langle ab||kj\rangle U _{ki}^{\lambda} + \frac{1}{2}\sum_{ijab}\sum_{f}(T _{ij}^{ab})^{*}\langle ab||fi\rangle U _{fi}^{\lambda} \nonumber \\
    &+ \frac{1}{2}\sum_{ijab}\sum_{k\neq i}T _{ij}^{ab}\langle kj||ab\rangle (-S _{ik}^{\lambda}-U _{ik}^{\lambda}) + \frac{1}{2}\sum_{ijab}\sum_{f}T _{ij}^{ab}\langle fj||ab\rangle (U _{fi}^{\lambda})^{*} \nonumber \\
    &+ \frac{1}{2}\sum_{ijab}\sum_{k}T _{ij}^{ab}\langle ij||kb\rangle(-S _{ak}^{\lambda}-(U _{ak}^{\lambda})^{*}) + \frac{1}{2}\sum_{ijab}\sum_{f\neq a}T _{ij}^{ab}\langle ij||fb\rangle U _{fa}^{\lambda} \nonumber \\
    &-\frac{1}{2}\sum_{ijab}T _{ij}^{ab}(T _{ij}^{ab})^{*}(\varepsilon _{i}^{\lambda}-\varepsilon _{a}^{\lambda}) + \text{AO terms}
\end{align}
collecting the $U _{af}^{\lambda}$ and $U _{fa}^{\lambda}$ terms and swapping some dummy indices:\\
\begin{align}
    A =&-\frac{1}{2}\sum_{ijab}\sum_{f\neq a} (T _{ij}^{ab})^{*}\langle fb||ij\rangle U _{af}^{\lambda} + \frac{1}{2} \sum_{ijab}\sum_{f\neq a}T _{ij}^{ab}\langle ij||fb\rangle U _{fa}^{\lambda} \nonumber \\
    =&- \frac{1}{2}\sum_{ijfb}\sum_{a\neq f}(T _{ij}^{fb})^{*}\langle ab||ij\rangle U _{fa}^{\lambda} + \frac{1}{2} \sum_{ijab}\sum_{f\neq a}T _{ij}^{ab}\langle ij||fb\rangle U _{fa}^{\lambda} \nonumber \\
    =& \frac{1}{2}\sum_{ijab}\sum_{f\neq a}\langle ij||fb\rangle \langle ab||ij\rangle U _{fa}^{\lambda}\Big(\frac{1}{\Delta _{ab}^{ij}}-\frac{1}{\Delta _{fb}^{ij}}\Big) \nonumber \\
    =& \frac{1}{2}\sum_{ijab}\sum_{f\neq a}\langle ij||fb\rangle \langle ab||ij\rangle U _{fa}^{\lambda}\frac{\epsilon _{a}-\epsilon _{f}}{\Delta _{ab}^{ij}\Delta _{fb}^{ij}}
\end{align}
using the expression for $U _{fa}^{\lambda}$:
\begin{align}
    A =& \frac{1}{2}\sum_{ijab}\sum_{f\neq a}\frac{\langle ij||fb\rangle\langle ab||ij\rangle(Q _{fa}^{\lambda}+\sum_{gm}[U _{gm}^{\lambda}\langle fm||ag\rangle + (U _{gm}^{\lambda})^{*}\langle fg||am\rangle])}{\Delta _{ab}^{ij}\Delta _{fb}^{ij}} \nonumber \\
    =& \frac{1}{2}\sum_{ijab}\sum_{f\neq a}T _{ij}^{ab}(T _{ij}^{fb})^{*}\Big(Q _{fa}^{\lambda}+\sum_{gm}[U _{gm}^{\lambda}\langle fm||ag\rangle + (U _{gm}^{\lambda})^{*}\langle fg||am\rangle]\Big)
\end{align}
evaluating the $\varepsilon _{a}^{\lambda}$ term in $\pdv{E ^{(2)}}{\lambda}$ expression:
\begin{align}
    \frac{1}{2}\sum_{ijab}T _{ij}^{ab}(T _{ij}^{ab})^{*}\varepsilon _{a}^{\lambda} =&\frac{1}{2}\sum_{ijab}T _{ij}^{ab}(T _{ij}^{ab})^{*}\Big(Q _{aa}^{\lambda} + \sum_{gm}[U _{gm}^{\lambda}\langle am||ag\rangle + (U _{gm}^{\lambda})^{*}\langle ag||am\rangle]\Big) \nonumber \\
    =& \frac{1}{2}\sum_{ijab}\sum_{f=a}T _{ij}^{ab}(T _{ij}^{fb})^{*}(Q _{fa}^{\lambda} + \sum_{gm}[U _{gm}^{\lambda}\langle fm||ag\rangle + (U _{gm}^{\lambda})^{*}\langle fg||am\rangle])
\end{align}
add this term into $A$:
\begin{equation}
    A + \frac{1}{2}\sum_{ijab}T _{ij}^{ab}(T _{ij}^{ab})^{*}\varepsilon _{a}^{\lambda} = \frac{1}{2}\sum_{ijabf}T _{ij}^{ab}(T _{ij}^{fb})^{*}\Big(Q _{fa}^{\lambda} + \sum_{gm}[U _{gm}^{\lambda}\langle fm||ag\rangle + (U _{gm}^{\lambda})^{*}\langle fg||am\rangle]\Big)
\end{equation}
Similarly, collecting the $U _{ki}^{\lambda}$ and $U _{ik}^{\lambda}$ terms, and add the $\varepsilon _{i}^{\lambda}$ term into them we get:
\begin{equation}
    -\frac{1}{2}\sum_{ijabk}(T _{ij}^{ab})^{*}T _{kj}^{ab}\Big(Q _{ki}^{\lambda} + \sum_{gm}[U _{gm}^{\lambda}\langle km||ig\rangle + (U _{gm}^{\lambda})^{*}\langle kg||im\rangle]\Big)
\end{equation}
Now looking at the $S _{ak}^{\lambda}$ terms:
\begin{align}
    &-\frac{1}{2}\sum_{ijab}\sum_{k}(T _{ij} ^{ab})^{*}\langle kb||ij\rangle S _{ak}^{\lambda} - \frac{1}{2}\sum_{ijab}\sum_{k}T _{ij}^{ab}\langle ij||kb\rangle S _{ak}^{\lambda} \nonumber \\
    =& -\frac{1}{2}\sum_{ijkab}S _{ak}^{\lambda}\Big(\frac{\langle ij||ab\rangle \langle kb||ij\rangle + \langle ab||ij\rangle \langle ij||kb\rangle}{\Delta _{ab}^{ij}}\Big)
\end{align}
\textcolor{blue}{no further simplification for general (complex) orbitals, but could be further simplified if assumed real orbitals}
\\

Now putting these all back into eqn (10):
\begin{align}
    \pdv{E ^{(2)}}{\lambda} =& -\frac{1}{2}\sum_{ijkab}S _{ak}^{\lambda}\Big(T _{ij}^{ab}\langle ij||kb\rangle + (T _{ij}^{ab})^{*}\langle kb||ij\rangle\Big) \nonumber \\
    &- \frac{1}{2}\sum_{ijab}\sum_{f\neq a}(T _{ij}^{ab})^{*}\langle fb||ij\rangle S _{af}^{\lambda} -\frac{1}{2}\sum_{ijab}\sum_{k\neq i}T _{ij}^{ab}\langle kj||ab\rangle S _{ik}^{\lambda}\nonumber \\
    &+\frac{1}{2}\sum_{ijab}\sum_{f}(T _{ij}^{ab})^{*}\langle ab||fi\rangle U _{fi}^{\lambda} + \frac{1}{2}\sum_{ijab}\sum_{f}T _{ij}^{ab}\langle fj||ab\rangle (U _{fi}^{\lambda})^{*} \nonumber \\
    &-\frac{1}{2}\sum_{ijab}\sum_{k}(T _{ij}^{ab})^{*}\langle kb||ij\rangle U _{ak}^{\lambda} - \frac{1}{2}\sum_{ijab}\sum_{k}T _{ij}^{ab}\langle ij||kb\rangle (U _{ak}^{\lambda})^{*} \nonumber \\
    &+ \frac{1}{2}\sum_{ijabf}T _{ij}^{ab}(T _{ij}^{fb})^{*}\Big(Q _{fa}^{\lambda} + \sum_{gm}[U _{gm}^{\lambda}\langle fm||ag\rangle + (U _{gm}^{\lambda})^{*}\langle fg||am\rangle]\Big) \nonumber \\
    &-\frac{1}{2}\sum_{ijabk}(T _{ij}^{ab})^{*}T _{kj}^{ab}\Big(Q _{ki}^{\lambda} + \sum_{gm}[U _{gm}^{\lambda}\langle km||ig\rangle + (U _{gm}^{\lambda})^{*}\langle kg||im\rangle]\Big)
\end{align}

By defining:
\begin{align}
    D _{ki} =& -\frac{1}{2}\sum_{jab}(T _{ij}^{ab})^{*}T _{kj}^{ab} \\
    D _{fa} =& \frac{1}{2}\sum_{ijb}(T _{ij}^{fb})^{*}T _{ij}^{ab} \\
    I _{ik} =& -\frac{1}{2}\sum_{jab}T _{ij}^{ab}\langle kj||ab\rangle \\
    I _{af} =& -\frac{1}{2}\sum_{ijb}(T _{ij}^{ab})^{*}\langle fb||ij\rangle \\
    I _{ak} =& -\frac{1}{2}\sum_{ijb}(T _{ij}^{ab}\langle ij||kb\rangle + (T _{ij}^{ab})^{*}\langle kb||ij\rangle)
\end{align}
the derivative becomes:
\begin{align}
    \pdv{E ^{(2)}}{\lambda} =& \sum_{ak}S _{ak}^{\lambda}I _{ak} + \sum_{a\neq f}S _{af}^{\lambda}I _{af} + \sum_{i\neq k}S _{ik}^{\lambda}I _{ik} \nonumber \\
    &+\sum_{af}D _{fa}Q _{fa}^{\lambda} + \sum_{ik}D _{ki}Q _{ki}^{\lambda} \nonumber \\
    &+ \frac{1}{2}\sum_{ijabf}(T _{ij}^{fb})^{*}\langle fb||ai\rangle U _{ai}^{\lambda} + \frac{1}{2}\sum_{ijabf}T _{ij}^{fb}\langle aj||fb\rangle (U _{ai}^{\lambda})^{*} \nonumber \\
    &- \frac{1}{2}\sum_{ijkab}(T _{kj}^{ab})^{*}\langle ib||kj\rangle U _{ai}^{\lambda} - \frac{1}{2}\sum_{ijkab}T _{kj}^{ab}\langle kj||ib\rangle (U _{ai}^{\lambda})^{*} \nonumber \\
    &+ \frac{1}{2}\sum_{ijmabfg}T _{mj}^{gb}(T _{mj}^{fb})^{*}U _{ai}^{\lambda}\langle fi||ga\rangle + \frac{1}{2}\sum_{ijmabfg}T _{mj}^{gb}(T _{mj}^{fb})^{*}(U _{ai}^{\lambda})^{*}\langle fa||gi\rangle \nonumber \\
    &- \frac{1}{2}\sum_{ijkmabg}(T _{mj}^{gb})^{*}T _{kj}^{gb}U _{ai}^{\lambda}\langle ki||ma\rangle - \frac{1}{2}\sum_{ijkmabg}(T _{mj}^{gb})^{*}T _{kj}^{gb}(U _{ai}^{\lambda})^{*}\langle ka||mi\rangle \nonumber \\
    =& \sum_{ak}S _{ak}^{\lambda}I _{ak} + \sum_{a\neq f}S _{af}^{\lambda}I _{af} + \sum_{i\neq k}S _{ik}^{\lambda}I _{ik} \nonumber \\
    &+\sum_{af}D _{fa}Q _{fa}^{\lambda} + \sum_{ik}D _{ki}Q _{ki}^{\lambda} \nonumber \\
    &+ \frac{1}{2}\sum_{ijabf}(T _{ij}^{fb})^{*}\langle fb||ai\rangle U _{ai}^{\lambda} + \frac{1}{2}\sum_{ijabf}T _{ij}^{fb}\langle aj||fb\rangle (U _{ai}^{\lambda})^{*} \nonumber \\
    &- \frac{1}{2}\sum_{ijkab}(T _{kj}^{ab})^{*}\langle ib||kj\rangle U _{ai}^{\lambda} - \frac{1}{2}\sum_{ijkab}T _{kj}^{ab}\langle kj||ib\rangle (U _{ai}^{\lambda})^{*} \nonumber \\
    &+\sum_{fg}\sum_{ai} D _{fg}\langle fi||ga\rangle U _{ai}^{\lambda} + \sum_{fg}\sum_{ai}D _{fg}\langle fa||gi\rangle (U _{ai}^{\lambda})^{*} \nonumber \\
    &+\sum_{km}\sum_{ai} D _{km}\langle ki||ma\rangle U _{ai}^{\lambda} + \sum_{km}\sum_{ai}D _{km}\langle ka||mi\rangle(U _{ai}^{\lambda})^{*} \nonumber \\
    =& \sum_{ai}S _{ai}^{\lambda}I _{ai} + \sum_{a\neq b}S _{a}^{\lambda}I _{ab} + \sum_{i\neq j}S _{ij}^{\lambda}I _{ij} + \sum_{ab}D _{ab}Q _{ab}^{\lambda} + \sum_{ij}D _{ij}Q _{ij}^{\lambda} \nonumber \\
    &+\frac{1}{2}\sum_{ai}\sum_{jbc}(T _{ij}^{bc})^{*}\langle bc||ai\rangle U _{ai}^{\lambda} + \frac{1}{2}\sum_{ai}\sum_{jbc}T _{ij}^{bc}\langle aj||bc\rangle (U _{ai} ^{\lambda})^{*} \nonumber \\
    &-\frac{1}{2}\sum_{ai}\sum_{jkb}(T _{kj}^{ab})^{*}\langle ib||kj\rangle U _{ai}^{\lambda} - \frac{1}{2}\sum_{ai}\sum_{jkb}T _{kj}^{ab}\langle kj||ib\rangle (U _{ai}^{\lambda})^{*} \nonumber \\
    &+\sum_{ai}\sum_{bc}D _{bc}\langle bi||ca\rangle U _{ai} ^{\lambda} + \sum_{ai}\sum_{bc}D _{bc}\langle ba||ci\rangle(U _{ai}^{\lambda})^{*} \nonumber \\
    &+\sum_{ai}\sum_{jk}D _{jk}\langle ji||ka\rangle U _{ai}^{\lambda} + \sum_{ai}\sum_{jk}D _{jk}\langle ja||ki\rangle (U _{ai}^{\lambda})^{*} \nonumber \\
    =& \sum_{ai}S _{ai}^{\lambda}I _{ai} + \sum_{ab}S _{ab}^{\lambda}I _{ab} + \sum_{ij}S _{ij}^{\lambda}I _{ij} + \sum_{ab}D _{ab}Q _{ab}^{\lambda} + \sum_{ij}D _{ij}Q _{ij}^{\lambda} \nonumber \\
    &+ \text{something like}\sum_{ai}X _{ai}U _{ai}^{\lambda}
\end{align}
\textcolor{red}{$\sum_{a\neq b}$ and $\sum_{i\neq j}$ terms, what about the $a=b$ and $i=j$ terms?} \\
\textcolor{blue}{Should I drop the complex conjugate? but still can't see how to merge $\langle bi||ca\rangle$ and $\langle ba||ci\rangle$ terms hence could not get the same $X _{ai}$ intermediate as in the article.}














\newpage
\section{Some Identities}
From CPHF orthonormality condition:
\begin{equation}
    U _{pq}^{\lambda} + (U _{qp}^{\lambda})^{*} + S _{pq}^{\lambda} = 0
\end{equation}
Consider the spin-orbital (and using $\mathbf{C}(\lambda) = \mathbf{C}(0)\mathbf{U}(\lambda)$):
\begin{align}
    |a \rangle = |\psi _{a}\rangle =& \sum_{\mu}C _{\mu a}(\lambda)|\phi _{\mu}\rangle \nonumber \\
    =& \sum_{\mu}\Big(\sum_{q}C _{\mu q}(0)U _{qa}(\lambda)\Big)|\phi _{\mu}\rangle \nonumber \\
    =& \sum_{\mu}\Big(\sum_{k}C _{\mu k}(0)U _{ka}(\lambda)\Big)|\phi _{\mu}\rangle + \sum_{\mu}\Big(\sum_{f\neq a}C _{\mu f}(0)U _{fa}(\lambda)\Big)|\phi _{\mu}\rangle
\end{align}
\textcolor{red}{Question: Why not include $U _{aa}$  into this sum?} \\
Taking derivative w.r.t. $\lambda$:
\begin{align}
    |a ^{\lambda}\rangle =& \sum_{\mu}\Big(\sum_{k}C _{\mu k}(0)U _{ka}^{\lambda}\Big)|\phi _{\mu}\rangle + \sum_{\mu}\Big(\sum_{f\neq a}C _{\mu f}(0)U _{fa}^{\lambda}\Big)|\phi _{\mu}\rangle \nonumber \\
    &+ \sum_{\mu}\Big(\sum_{k}C _{\mu k}(0)U _{ka}\Big)|\phi _{\mu}^{\lambda}\rangle + \sum_{\mu}\Big(\sum_{f\neq a}C _{\mu f}(0)U _{fa}\Big)|\phi _{\mu}^{\lambda}\rangle
\end{align}
Noticing that $\mathbf{U}(0)=\mathbf{I}$ hence $\sum_{\mu}C _{\mu k}(0)|\phi _{\mu}\rangle = |\psi _{k}\rangle$:
\begin{align}
    |a ^{\lambda}\rangle =& \sum_{k}U _{ka}^{\lambda}|\psi _{k}\rangle + \sum_{f\neq a}U _{fa}^{\lambda}|\psi _{f}\rangle + \sum_{\mu q}C _{\mu _{q}}(0)U _{qa}|\phi _{\mu}^{\lambda}\rangle \nonumber \\
    =& \sum_{k}U _{ka}^{\lambda}|k\rangle + \sum_{f\neq a}U _{fa}^{\lambda}|f\rangle + \sum_{\mu}C _{\mu a}|\mu ^{\lambda}\rangle
\end{align}

Similarly:
\begin{align}
    |i ^{\lambda}\rangle = \sum_{k\neq i}U _{ki}^{\lambda}|k\rangle + \sum_{f}U _{fi}^{\lambda}|f\rangle + \sum_{\mu}C _{\mu i}|\mu ^{\lambda}\rangle
\end{align}

Expression for CPHF coefficients (c.f. Pople et al. 1979): 
\begin{equation}
    U _{fa}^{\lambda} = \frac{1}{\varepsilon _{a}-\varepsilon _{f}}(Q _{fa}^{\lambda} + \sum_{gm}[U _{gm}^{\lambda}\langle fm||ag\rangle + (U _{gm}^{\lambda})^{*}\langle fg||am\rangle])
\end{equation}
\begin{equation}
    U _{ki}^{\lambda} = \frac{1}{\varepsilon _{i}-\varepsilon _{k}}(Q _{ki}^{\lambda} + \sum_{gm}[U _{gm}^{\lambda}\langle fm||ag\rangle + (U _{gm}^{\lambda})^{*}\langle kg||im\rangle])
\end{equation}
\begin{equation}
    \varepsilon _{a}^{\lambda} = Q _{aa}^{\lambda} + \sum_{gm}[U _{gm}^{\lambda}\langle am||ag\rangle + (U _{gm}^{\lambda})^{*}\langle ag||am\rangle]
\end{equation}
\begin{equation}
    \varepsilon _{i}^{\lambda} = Q _{ii}^{\lambda} + \sum_{gm}[U _{gm}^{\lambda}\langle im||ig\rangle + (U _{gm}^{\lambda})^{*}\langle ig||im\rangle]
\end{equation}





\end{document}