\documentclass[a4paper,11pt]{article}
\usepackage{braket}
\usepackage{physics}
\usepackage{parskip}
\usepackage{bm}
\usepackage{float}
\usepackage[utf8]{inputenc}
\usepackage{amsmath}
\usepackage{pgfplots}
\usepackage{mathrsfs}
\usepackage{simpler-wick}
\usepackage{enumerate}
\usepackage{csquotes}
\usepackage{subcaption}
\usepackage{fancyhdr}
\usepackage{tablefootnote}
\usepackage{microtype}
\usepackage{cleveref}
\usepackage{titling}
\usepackage{erewhon}
\usepackage[a4paper,width=150mm,top=25mm,bottom=25mm]{geometry}
\usepackage[Sonny]{fncychap}
\usepackage[calcwidth]{titlesec}
\usepackage[makeroom]{cancel}

\usetikzlibrary{shapes.geometric, arrows}

\allowdisplaybreaks

\pgfplotsset{compat=1.7}

%fncychap layout (for chapter page)
%\renewcommand{\thechapter}{\Roman{chapter}}
\ChNameVar{\bfseries\LARGE\fontfamily{phv}}
\ChNumVar{\fontsize{50}{52}\usefont{OT1}{ptm}{m}{n}\selectfont}
\ChTitleVar{\LARGE\rm\bfseries}
\ChRuleWidth{0.8pt}

%fancyhdr layout (for header and footer)
\pagestyle{fancy}
\fancyhead{}
\fancyhead[C]{\fontsize{9}{9}\itshape{\rightmark}}
\setlength{\headheight}{15pt}

\begin{document}
\subsection{Perturbed Brillouin Condition}
The SCF density matrix is defined as:
\begin{equation}
    D _{\mu \nu}^{\text{SCF}} = \sum_{i}^{N} C _{\mu i}^{*}C _{\nu i}
\end{equation}
in which the MO coefficients are parameterized as:
\begin{align}
    C _{\mu p}(\lambda) =& \sum_{q} C _{\mu q}(0)U(\lambda)_{qp} \\
    \mathbf{C}(\lambda) =& \mathbf{C}(0)\mathbf{U}(\lambda)
\end{align}


Define the one- and two-electron parts of the fock matrix, in AO and MO basis, as:
\begin{equation}
    \begin{aligned}[t]
     h _{pq}=& \langle p|\hat{h}|q\rangle
     = \sum_{\mu \nu}C _{\mu p}^{*}h _{\mu \nu}^{\text{AO}}C _{\nu q}\\
     h _{\mu \nu} ^{\text{AO}}=& \langle \mu|\hat{h}|\nu\rangle \\
    \mathbf{h} =& \mathbf{C}^{\dagger}\mathbf{h}^{\text{AO}}\mathbf{C} \\
    \end{aligned}
    \qquad 
    \begin{aligned}[t]
     g _{pq}=& \sum_{i}\langle pi||qi\rangle
     = \sum_{i}\sum_{\mu \nu}C _{\mu p}^{*}\langle \mu i||\nu i\rangle C _{\nu q}\\
     g _{\mu \nu}^{\text{AO}}=& \sum_{i}\langle \mu i||\nu i\rangle
     = \sum_{\rho \sigma}D _{\rho \sigma}\langle \mu \rho||\nu \sigma\rangle \\
    \mathbf{g} =& \mathbf{C}^{\dagger}\mathbf{g}^{\text{AO}}\mathbf{C} \\
    \end{aligned}
\end{equation}
Therefore, the Fock matrix could be expressed as (with the dependency on SCF density explicitly addressed):
\begin{align}
    f _{pq} =& h _{pq} + \sum_{i}\langle pi||qi\rangle \nonumber \\
    =& \sum_{\mu \nu}C _{\mu p}^{*}h _{\mu \nu}^{\text{AO}}C _{\nu q} + \sum_{\mu \nu}C _{\mu p}^{*} g _{\mu \nu}^{\text{AO}} C _{\nu q} \nonumber \\
    =& \sum_{\mu \nu}C _{\mu p}^{*}\langle \mu|\hat{h}|\nu\rangle C _{\nu q} + \sum_{\mu \nu}C _{\mu p}^{*}\big(\sum_{\rho \sigma} D _{\rho \sigma}\langle \mu \rho||\nu \sigma\rangle\big)C _{\nu q} \\
    f ^{\text{AO}}_{\mu \nu} =& h _{\mu \nu}^{\text{AO}} + g ^{\text{AO}}_{\mu \nu} = \langle \mu|\hat{h}|\nu\rangle + \sum_{\rho \sigma}D _{\rho \sigma}\langle \mu \rho||\nu \sigma\rangle \\
    \mathbf{f}=& \mathbf{h} + \mathbf{g}[\mathbf{D}^{\text{SCF}}] \nonumber \\
    =& \mathbf{C}^{\dagger}\mathbf{h}^{\text{AO}}\mathbf{C} + \mathbf{C}^{\dagger}\mathbf{g}^{\text{AO}}[\mathbf{D}^{\text{SCF}}]\mathbf{C} \nonumber \\
    =& \mathbf{C}^{\dagger}\mathbf{F}^{\text{AO}}[\mathbf{D}^{\text{SCF}}]\mathbf{C} \\
    \mathbf{f}^{\text{AO}}[\mathbf{D}^{\text{SCF}}] =& \mathbf{h}^{\text{AO}} + \mathbf{g}^{\text{AO}}[\mathbf{D}^{\text{SCF}}]
\end{align}
Evaluating the derivative at $\lambda = 0$, noting that $\mathbf{U}(0) = \mathbf{I}$:
\begin{align}
    \mathbf{f}^{\lambda} =& \frac{\dd{\mathbf{f}(\lambda)}}{\dd{\lambda}}\Big|_{{\lambda = 0}} = \Big(\mathbf{C}^{\dagger}(\lambda)\mathbf{f}^{\text{AO}}[\mathbf{D}^{\text{SCF}}(\lambda)](\lambda)\mathbf{C}(\lambda)\Big)^{\lambda} \nonumber \\
    =&\mathbf{C}^{\lambda \dagger}(\lambda)\mathbf{f}^{\text{AO}}[\mathbf{D}^{\text{SCF}}(\lambda)](\lambda)\mathbf{C}(\lambda) + \mathbf{C}^{\dagger}(\lambda)\mathbf{f}^{\text{AO}}[\mathbf{D}^{\text{SCF}}(\lambda)](\lambda)\mathbf{C}^{\lambda}(\lambda) \nonumber \\
    &+ \mathbf{C}^{\dagger}(\lambda) \Big(\mathbf{h}^{\text{AO}}(\lambda) + \mathbf{g}^{\text{AO}}[\mathbf{D}^{\text{SCF}}(\lambda)](\lambda)\Big)^{\lambda} \mathbf{C}(\lambda)  \nonumber \\
    =& \mathbf{U}^{\lambda \dagger}(\lambda)\underbrace{\mathbf{U}^{\dagger}(0)\mathbf{C}^{\dagger}(0)}_\text{$\mathbf{C}^{\dagger}(\lambda = 0)$}\mathbf{f}^{\text{AO}}[\mathbf{D}^{\text{SCF}}(\lambda)](\lambda)\mathbf{C}(\lambda) + \mathbf{C}^{\dagger}(\lambda)\mathbf{f}^{\text{AO}}[\mathbf{D}^{\text{SCF}}(\lambda)](\lambda)\underbrace{\mathbf{C}(0)\mathbf{U}(0)}_\text{$\mathbf{C}(\lambda = 0)$}\mathbf{U}^{\lambda}(\lambda) \nonumber \\
    &+ \mathbf{C}^{\dagger}(\lambda)\Big(\mathbf{h}^{\text{AO},\lambda}(\lambda) + \mathbf{g}^{\text{AO}, \lambda}[\mathbf{D}^{\text{SCF}}(\lambda)](\lambda) + \mathbf{g}^{\text{AO}}[\mathbf{D}^{\text{SCF},\lambda}(\lambda)](\lambda)\Big)\mathbf{C}(\lambda) \nonumber \\
    =& \mathbf{U}^{\lambda \dagger}\mathbf{f} + \mathbf{f}\mathbf{U}^{\lambda} + \mathbf{C}^{\dagger}\mathbf{h}^{\text{AO}, \lambda}\mathbf{C}
    + \mathbf{C}^{\dagger}\mathbf{g}^{\text{AO},\lambda}[\mathbf{D}^{\text{SCF}}]\mathbf{C} + \mathbf{C}^{\dagger}\mathbf{g}^{\text{AO}}[\mathbf{D}^{\text{SCF},\lambda}]\mathbf{C}
\end{align}
The perturbed Brillouin condition is:
\begin{equation}
    f _{ai}^{\lambda} = 0
\end{equation}
To evaluate the perturbed Fock matrix, we write the perturbed quantities in suffix notation as (assuming canonical orbitals, i.e. $f _{pq} = \delta _{pq}\varepsilon _{p}$):
\begin{align}
    (\mathbf{U}^{\lambda \dagger}\mathbf{f}) _{ai} =& U ^{\lambda *}_{ia}\varepsilon _{i} = \frac{\dd{U _{ia}^{*}}}{\dd{\lambda}}\Big|_{{\lambda = 0}}\varepsilon _{i} \\
    (\mathbf{f}\mathbf{U}^{\lambda})_{ai} =& \varepsilon _{a}U _{ai}^{\lambda} = \varepsilon _{a}\frac{\dd{U _{ai}}}{\dd{\lambda}}\Big|_{{\lambda=0}} \\
    (\mathbf{C}^{\dagger}\mathbf{h}^{\text{AO},\lambda}\mathbf{C})_{ai}=&\sum_{\mu \nu}C _{\mu a}^{*}h _{\mu \nu}^{\lambda} C _{\nu i} = \sum_{\mu \nu}C _{\nu a}^{*}\frac{\dd{h _{\mu \nu}}}{\dd{\lambda}}\Big|_{{\lambda=0}}C _{\nu i} \\
    (\mathbf{C}^{\dagger}\mathbf{g}^{\text{AO}, \lambda}[\mathbf{D}^{\text{SCF}}]\mathbf{C})_{ai} =& \sum_{\mu \nu}C _{\mu a}^{*}(\sum_{\rho \sigma}D _{\rho \sigma}\langle \mu \rho||\nu \sigma\rangle ^{\lambda})C _{\nu i} \nonumber \\
    =& \sum_{\mu \nu}C _{\mu a}^{*}(\sum_{\rho \sigma}D _{\rho \sigma}\frac{\dd{\langle \mu \rho||\nu \sigma\rangle}}{\dd{\lambda}}\Big|_{{\lambda=0}})C _{\nu i} \\
    (\mathbf{C}^{\dagger}\mathbf{g}^{\text{AO}}[\mathbf{D}^{\text{SCF},\lambda}]\mathbf{C})_{ai} =& \sum_{\mu \nu}C _{\mu a}^{*}(\sum_{\rho \sigma}D _{\rho \sigma}^{\lambda}\langle \mu \rho||\nu \sigma\rangle)C _{\nu i} \nonumber \\
    =& \sum_{\mu \nu} C _{\mu a}^{*}(\sum_{\rho \sigma}\frac{\dd{D}_{\rho \sigma}}{\dd{\lambda}}\Big|_{{\lambda=0}}\langle \mu \rho||\nu \sigma\rangle)C _{\nu i}
\end{align}





\end{document}